Coq/src/SimRel.v
@@ -514,3 +514,97 @@ Section SimRel.
   End SimRelCommonProps.
 
 End SimRel.
+
+Section SimRelLemmas.
+
+  Variable prog : Prog.t.
+  Variable S : ES.t.
+  Variable G : execution.
+  Variable sc : relation actid.
+  Variable TC : trav_config.
+  Variable f : actid -> eventid.
+
+  Notation "'SE'" := S.(ES.acts_set).
+  Notation "'SEinit'" := S.(ES.acts_init_set).
+  Notation "'SEninit'" := S.(ES.acts_ninit_set).
+  Notation "'Stid'" := (S.(ES.tid)).
+  Notation "'Slab'" := (S.(ES.lab)).
+  Notation "'Sloc'" := (loc S.(ES.lab)).
+  Notation "'K'" := S.(ES.cont_set).
+
+  Notation "'STid' t" := (fun x => Stid x = t) (at level 1).
+
+  Notation "'SR'" := (fun a => is_true (is_r Slab a)).
+  Notation "'SW'" := (fun a => is_true (is_w Slab a)).
+  Notation "'SF'" := (fun a => is_true (is_f Slab a)).
+  Notation "'SRel'" := (fun a => is_true (is_rel Slab a)).
+
+  Notation "'Ssb'" := (S.(ES.sb)).
+  Notation "'Scf'" := (S.(ES.cf)).
+  Notation "'Srmw'" := (S.(ES.rmw)).
+  Notation "'Sjf'" := (S.(ES.jf)).
+  Notation "'Sjfi'" := (S.(ES.jfi)).
+  Notation "'Sjfe'" := (S.(ES.jfe)).
+  Notation "'Srf'" := (S.(ES.rf)).
+  Notation "'Srfi'" := (S.(ES.rfi)).
+  Notation "'Srfe'" := (S.(ES.rfe)).
+  Notation "'Sco'" := (S.(ES.co)).
+  Notation "'Sew'" := (S.(ES.ew)).
+
+  Notation "'Srs'" := (S.(Consistency.rs)).
+  Notation "'Srelease'" := (S.(Consistency.release)).
+  Notation "'Ssw'" := (S.(Consistency.sw)).
+  Notation "'Shb'" := (S.(Consistency.hb)).
+
+  Notation "'thread_syntax' tid"  := 
+    (Language.syntax (thread_lts tid)) (at level 10, only parsing).  
+
+  Notation "'thread_st' tid" := 
+    (Language.state (thread_lts tid)) (at level 10, only parsing).
+
+  Notation "'thread_init_st' tid" := 
+    (Language.init (thread_lts tid)) (at level 10, only parsing).
+  
+  Notation "'thread_cont_st' tid" :=
+    (fun st => existT _ (thread_lts tid) st) (at level 10, only parsing).
+
+  Notation "'GE'" := G.(acts_set).
+  Notation "'GEinit'" := (is_init ∩₁ GE).
+  Notation "'GEninit'" := ((set_compl is_init) ∩₁ GE).
+
+  Notation "'Gtid'" := (tid).
+  Notation "'Glab'" := (G.(lab)).
+  Notation "'Gloc'" := (loc G.(lab)).
+  
+  Notation "'GTid' t" := (fun x => tid x = t) (at level 1).
+  Notation "'GNTid' t" := (fun x => tid x <> t) (at level 1).
+
+  Notation "'GR'" := (fun a => is_true (is_r Glab a)).
+  Notation "'GW'" := (fun a => is_true (is_w Glab a)).
+  Notation "'GF'" := (fun a => is_true (is_f Glab a)).
+
+  Notation "'GRel'" := (fun a => is_true (is_rel Glab a)).
+  
+  Notation "'Gsb'" := (G.(sb)).
+  Notation "'Grmw'" := G.(rmw).
+  Notation "'Grf'" := (G.(rf)).
+  Notation "'Gco'" := (G.(co)).
+
+  Notation "'Grs'" := (G.(imm_s_hb.rs)).
+  Notation "'Grelease'" := (G.(imm_s_hb.release)).
+  Notation "'Ghb'" := (G.(imm_s_hb.hb)).
+
+  Notation "'C'"  := (covered TC).
+  Notation "'I'"  := (issued TC).
+
+  Notation "'Gvf'" := (furr G sc).
+
+  Lemma simrel_init 
+        (nInitProg : ~ IdentMap.In tid_init prog)
+        (PExec : program_execution prog G)
+        (WF : Execution.Wf G)
+        (CONS : imm_consistent G sc) : 
+    simrel_common prog (ES.init prog) G sc (init_trav G) a2e_init.
+  Proof. clear S TC f. admit. Admitted.
+
+End SimRelLemmas.
