Coq/src/SimRelStep.v
@@ -1,0 +1,145 @@
+Require Import Omega.
+Require Import Program.Basics.
+Require Import Coq.Logic.FunctionalExtensionality Classical_Prop.
+From hahn Require Import Hahn.
+From promising Require Import Basic.
+From imm Require Import Events Execution
+     Traversal TraversalConfig SimTraversal SimTraversalProperties
+     Prog ProgToExecution ProgToExecutionProperties Receptiveness
+     imm_common imm_s imm_s_hb SimulationRel
+     CertExecution2 CertExecutionMain
+     SubExecution CombRelations AuxRel.
+Require Import AuxRel AuxDef EventStructure BasicStep Step StepWf Consistency 
+        LblStep CertRf CertGraph EventToAction ImmProperties
+        SimRelCont SimRelEventToAction SimRel SimRelCert 
+        SimRelCertBasicStep SimRelCertStep.  
+
+Set Implicit Arguments.
+Local Open Scope program_scope.
+
+Section SimRelStep.
+
+  Variable prog : Prog.t.
+  Variable G : execution.
+  Variable sc : relation actid.
+  Variable TC : trav_config.
+  Variable TC' : trav_config.
+  Variable f : actid -> eventid.
+  Variable h : actid -> eventid.
+
+  Notation "'SE' S" := S.(ES.acts_set) (at level 10).
+  Notation "'SEinit' S" := S.(ES.acts_init_set) (at level 10).
+  Notation "'SEninit' S" := S.(ES.acts_ninit_set) (at level 10).
+  Notation "'Stid' S" := (S.(ES.tid)) (at level 10).
+  Notation "'Slab' S" := S.(ES.lab) (at level 10).
+  Notation "'Sloc' S" := (loc S.(ES.lab)) (at level 10).
+
+  Notation "'Ssb' S" := S.(ES.sb) (at level 10).
+  Notation "'Srmw' S" := S.(ES.rmw) (at level 10).
+  Notation "'Sew' S" := S.(ES.ew) (at level 10).
+  Notation "'Sjf' S" := S.(ES.jf) (at level 10).
+  Notation "'Srf' S" := S.(ES.rf) (at level 10).
+  Notation "'Sco' S" := S.(ES.co) (at level 10).
+  Notation "'Scf' S" := S.(ES.cf) (at level 10).
+
+  Notation "'Sjfe' S" := S.(ES.jfe) (at level 10).
+  Notation "'Srfe' S" := S.(ES.rfe) (at level 10).
+  Notation "'Scoe' S" := S.(ES.coe) (at level 10).
+  Notation "'Sjfi' S" := S.(ES.jfi) (at level 10).
+  Notation "'Srfi' S" := S.(ES.rfi) (at level 10).
+  Notation "'Scoi' S" := S.(ES.coi) (at level 10).
+
+  Notation "'Scc' S" := S.(cc) (at level 10).
+  Notation "'Ssw' S" := S.(sw) (at level 10).
+  Notation "'Shb' S" := S.(hb) (at level 10).
+  Notation "'Secf' S" := (S.(Consistency.ecf)) (at level 10).
+  Notation "'Seco' S" := (Consistency.eco S Weakestmo) (at level 10).
+
+  Notation "'SR' S" := (fun a => is_true (is_r S.(ES.lab) a)) (at level 10).
+  Notation "'SW' S" := (fun a => is_true (is_w S.(ES.lab) a)) (at level 10).
+  Notation "'SF' S" := (fun a => is_true (is_f S.(ES.lab) a)) (at level 10).
+
+  Notation "'SPln' S" := (fun a => is_true (is_only_pln S.(ES.lab) a)) (at level 10).
+  Notation "'SRlx' S" := (fun a => is_true (is_rlx S.(ES.lab) a)) (at level 10).
+  Notation "'SRel' S" := (fun a => is_true (is_rel S.(ES.lab) a)) (at level 10).
+  Notation "'SAcq' S" := (fun a => is_true (is_acq S.(ES.lab) a)) (at level 10).
+  Notation "'SAcqrel' S" := (fun a => is_true (is_acqrel S.(ES.lab) a)) (at level 10).
+  Notation "'SSc' S" := (fun a => is_true (is_sc S.(ES.lab) a)) (at level 10).
+
+  Notation "'K' S" := (S.(ES.cont_set)) (at level 10).
+
+  Notation "'Stid_' t" := (fun x => Stid x = t) (at level 1).
+
+  Notation "'GE'" := G.(acts_set).
+  Notation "'GEinit'" := (is_init ∩₁ GE).
+  Notation "'GEninit'" := ((set_compl is_init) ∩₁ GE).
+  Notation "'Glab'" := (G.(lab)).
+  Notation "'Gtid'" := (tid).
+  Notation "'Grmw'" := G.(rmw).
+  Notation "'Gaddr'" := G.(addr).
+  Notation "'Gdata'" := G.(data).
+  Notation "'Gctrl'" := G.(ctrl).
+  Notation "'Grmw_dep'" := G.(rmw_dep).
+
+  Notation "'Gtid_' t" := (fun x => tid x = t) (at level 1).
+  Notation "'GNtid_' t" := (fun x => tid x <> t) (at level 1).
+
+  Notation "'Tid_' t" := (fun x => tid x = t) (at level 1).
+  Notation "'NTid_' t" := (fun x => tid x <> t) (at level 1).
+
+  Notation "'GR'" := (fun a => is_true (is_r Glab a)).
+  Notation "'GW'" := (fun a => is_true (is_w Glab a)).
+  Notation "'GR_ex'" := (fun a => R_ex Glab a).
+
+  Notation "'Gsb'" := (G.(sb)).
+  Notation "'Ghb'" := (G.(imm_s_hb.hb)).
+  Notation "'Grf'" := (G.(rf)).
+  Notation "'Gco'" := (G.(co)).
+  Notation "'Gvf'" := (G.(furr)).
+  Notation "'Gppo'" := (G.(ppo)).
+
+  Notation "'C'"  := (covered TC).
+  Notation "'I'"  := (issued TC).
+  Notation "'C''"  := (covered TC').
+  Notation "'I''"  := (issued TC').
+
+  Notation "'thread_syntax' tid"  := 
+    (Language.syntax (thread_lts tid)) (at level 10, only parsing).  
+
+  Notation "'thread_st' tid" := 
+    (Language.state (thread_lts tid)) (at level 10, only parsing).
+
+  Notation "'thread_init_st' tid" := 
+    (Language.init (thread_lts tid)) (at level 10, only parsing).
+
+  Notation "'thread_cont_st' tid" :=
+    (fun st => existT _ (thread_lts tid) st) (at level 10, only parsing).
+
+  Notation "'cont_lang'" :=
+    (fun S k => thread_lts (ES.cont_thread S k)) (at level 10, only parsing).
+  
+  Lemma simrel_cert_start S thread
+        (SRC : simrel_common prog S G sc TC f) 
+        (ITRAV_STEP : isim_trav_step G sc thread TC TC') :
+    exists k st st', 
+      ⟪ kTID : thread = ES.cont_thread S k ⟫ /\      
+      ⟪ SRCC : simrel_cert prog S G sc TC TC' f f k st st' ⟫.
+  Proof. admit. Admitted.
+
+  Lemma simrel_cert_end S k 
+        (st : thread_st (ES.cont_thread S k))
+        (SRCC : simrel_cert prog S G sc TC TC' f h k st st) :
+    simrel_common prog S G sc TC' h.
+  Proof. admit. Admitted.
+  
+  Lemma simrel_step S 
+        (SRC : simrel_common prog S G sc TC f) 
+        (TRAV_STEP : sim_trav_step G sc TC TC') :
+    exists S' f', 
+      ⟪ STEPS : (ESstep.t Weakestmo)＊ S S' ⟫ /\      
+      ⟪ SRC' : simrel_common prog S' G sc TC' f' ⟫.
+  Proof. 
+    
+    admit. Admitted.
+  
+End SimRelStep.
